PPlusProperties.v
@@ -832,7 +832,7 @@ Proof.
 Qed.
 
 Definition called_by (f : DefMethT) (call :MethT) : bool :=
-  (getBool (prod_dec string_dec Signature_dec' (fst f, projT1 (snd f)) (fst call, projT1 (snd call)))).
+  (getBool (prod_dec string_dec Signature_dec (fst f, projT1 (snd f)) (fst call, projT1 (snd call)))).
 
 Local Notation complement f := (fun x => negb (f x)).
 
@@ -978,7 +978,7 @@ Lemma PSemAction_inline_In (f : DefMethT) o:
       PSemAction o (inlineSingle f a) (readRegs' ++ readRegs) (newRegs' ++ newRegs) (calls'++calls2) retV2.
 Proof.
   induction a; intros.
-  - simpl; destruct (fst f =? meth) eqn:G; [rewrite String.eqb_eq in G|rewrite eqb_neq in G]; [destruct Signature_dec' | ]; subst.
+  - simpl; destruct (fst f =? meth) eqn:G; [rewrite String.eqb_eq in G|rewrite eqb_neq in G]; [destruct Signature_dec | ]; subst.
     + inv H0; EqDep_subst.
       assert (In (fst f, existT SignT (projT1 (snd f)) (evalExpr e, mret)) calls1).
       { case (in_app_or _ _ _ (Permutation_in _ (Permutation_sym (HAcalls)) (in_eq _ _)));
@@ -1585,7 +1585,7 @@ Proof.
   unfold MatchingExecCalls_flat.
   induction calls; intros.
   - simpl; exists execs; reflexivity.
-  - destruct (prod_dec string_dec Signature_dec' (fst f, projT1 (snd f)) (fst a, projT1 (snd a))).
+  - destruct (prod_dec string_dec Signature_dec (fst f, projT1 (snd f)) (fst a, projT1 (snd a))).
     + specialize (in_map (fun x => (fst x, projT1 (snd x))) _ _ H) as P1; simpl in P1; rewrite e in P1.
       specialize (H0 a P1) as P2.
       rewrite getNumFromCalls_eq_cons in P2; auto.
@@ -2108,7 +2108,7 @@ Lemma WfActionT_inline_Rule_inline_action (k : Kind) m (a : ActionT type k) rn (
 Proof.
   induction 1; try econstructor; eauto.
   simpl.
-  destruct String.eqb; [destruct Signature_dec'|]; subst; econstructor; eauto.
+  destruct String.eqb; [destruct Signature_dec|]; subst; econstructor; eauto.
   econstructor.
   intros.
   specialize (H1 v).
@@ -2939,7 +2939,7 @@ Lemma WfActionT_inline_Meth_inline_action (k : Kind) m (a : ActionT type k) gn (
 Proof.
   induction 1; try econstructor; eauto.
   simpl.
-  destruct String.eqb;[destruct Signature_dec'|]; subst; econstructor; eauto.
+  destruct String.eqb;[destruct Signature_dec|]; subst; econstructor; eauto.
   econstructor.
   intros.
   specialize (H1 v).
@@ -4092,7 +4092,7 @@ Section flatten_and_inline_all.
     inv H0; [inv H1; contradiction|].
     inv HStep.
     apply Trace_TraceHide' in HOldTrace; dest.
-    destruct (in_dec (prod_dec string_dec Signature_dec') (s, projT1 v)
+    destruct (in_dec (prod_dec string_dec Signature_dec) (s, projT1 v)
                      (getKindAttr (getAllMethods m))).
     - inv H1.
       specialize (HHidden _ i).
@@ -4533,7 +4533,7 @@ Lemma Step_HideMeth_removeMeth_noCalls (f : string) (m : BaseModule) (o : RegsT)
 Proof.
   intros; inv H.
   apply Step_removeMeth; auto; intros.
-  destruct (in_dec (prod_dec string_dec Signature_dec')
+  destruct (in_dec (prod_dec string_dec Signature_dec)
                    (f, projT1 v) (getKindAttr (getMethods m))).
   - specialize (HHidden _ i); specialize (H0 v).
     unfold getListFullLabel_diff in HHidden.
@@ -5072,7 +5072,7 @@ Lemma PSemAction_In_inline (f : DefMethT) o:
 Proof.
   intros retK2 a.
   induction a; subst; simpl in *; intros.
-  - destruct String.eqb eqn:G;[destruct Signature_dec'|]; subst; simpl in *.
+  - destruct String.eqb eqn:G;[destruct Signature_dec|]; subst; simpl in *.
     + inv H0; EqDep_subst.
       inv HPSemAction; EqDep_subst.
       specialize (H _ _ _ _ _ HPSemActionCont); dest.
@@ -7441,7 +7441,7 @@ Lemma WfConcatActionT_inlineSingle_Meth {k : Kind} (f: DefMethT) (a : ActionT ty
 Proof.
   intros.
   induction a; unfold inlineSingle; inv H0; EqDep_subst; try econstructor; eauto.
-  destruct String.eqb;[destruct Signature_dec'|]; subst; simpl in *; econstructor; eauto.
+  destruct String.eqb;[destruct Signature_dec|]; subst; simpl in *; econstructor; eauto.
   econstructor; eauto.
 Qed.
 
